Reformatação de tudo* que fora feito

DFA.v
@@ -4,19 +4,14 @@ Require BinIntDef.
 
 Definition state := nat.
 
-Definition states_num := 6.
-(* Axiom states_num : nat. *)
+Axiom states_num_minus_1 : nat.
+(* Definition states_num_minus_1 := 5. *)
+
+Definition states_num := S states_num_minus_1.
 
 Inductive event := add | rem | oth.
 
-Definition count_event e :=
-  match e with
-    add =>   1%Z  |
-    rem => (-1)%Z |
-    oth =>   0%Z
-  end.
-
-Definition transition (q:state) e :=
+(* Definition transition (q:state) e :=
   match q, e with
     0, add => 5 |
     0, rem => 1 |
@@ -26,13 +21,14 @@ Definition transition (q:state) e :=
     4, rem => 1 |
     5, add => 1 |
     _,  _  => 10
-  end.
-(* Axiom transition : state->event->state. *)
+  end. *)
+Axiom transition : state->event->state.
 
-Definition is_marked (q:state) :=
+(* Definition is_marked (q:state) :=
   match q with
     _ => false
-  end.
+  end. *)
+Axiom is_marked : state->bool.
 
 Definition DFA := (states_num, transition, is_marked).
 
@@ -55,12 +51,43 @@ Fixpoint xtransition q w :=
     []  => q
   end.
 
-Definition is_generated w := ~ is_sink_state (xtransition 0 w).
+Definition ixtransition w := xtransition 0 w.
+
+Lemma ixtransition_nil__0 : ixtransition [] = 0.
+Proof.
+  unfold ixtransition.
+  reflexivity.
+Qed.
+
+Definition is_proper_transition q e := ~ is_sink_state (xtransition q [e]).
+
+Definition is_generated w := ~ is_sink_state (ixtransition w).
 
 Lemma is_sink_stateb__is_sink_state : forall q,
   is_sink_stateb q = true <-> is_sink_state q.
 Proof.
-Admitted.
+  intro q.
+  split; intro H.
+  - apply leb_complete, H.
+  - apply leb_correct, H.
+Qed.
+
+Lemma isnt_sink_stateb__isnt_sink_state : forall q,
+  is_sink_stateb q = false <-> ~ is_sink_state q.
+Proof.
+  intro q.
+  split; intro H.
+  - unfold not.
+    intro contra.
+    apply is_sink_stateb__is_sink_state in contra.
+    rewrite H in contra.
+    discriminate contra.
+  - unfold is_sink_state in H.
+    unfold is_sink_stateb.
+    apply leb_iff_conv.
+    apply not_ge in H.
+    apply H.
+Qed.
 
 Lemma xtransition_sink_state : forall w q,
   is_sink_stateb q = true -> xtransition q w = q.
@@ -87,10 +114,18 @@ Proof.
     + apply IHw.
 Qed.
 
-Theorem prefix_closed: forall w w',
+Theorem ixtransition_distr : forall w w',
+  ixtransition (w ++ w') = xtransition (ixtransition w) w'.
+Proof.
+  intros w w'.
+  unfold ixtransition.
+  apply xtransition_distr.
+Qed.
+
+Theorem prefix_closed : forall w w',
   is_generated (w ++ w') -> is_generated w.
 Proof.
-  unfold is_generated, not.
+  unfold is_generated, ixtransition, not.
   intros w w' H H0.
   rewrite xtransition_distr in H.
   apply is_sink_stateb__is_sink_state in H0.
