QueueingSystems.v
@@ -3,13 +3,124 @@ Import ListNotations Coq.Bool.Bool.
 Require BinIntDef.
 Local Open Scope Z_scope.
 
+Definition count_event e :=
+  match e with
+    add =>   1%Z  |
+    rem => (-1)%Z |
+    oth =>   0%Z
+  end.
+
+Fixpoint count_buffer w :=
+  match w with
+     []  => 0                             |
+    e::w => count_event e + count_buffer w
+  end.
+
+Lemma count_buffer_distr : forall w1 w2,
+  count_buffer (w1 ++ w2) = count_buffer w1 + count_buffer w2.
+Proof.
+  intros w1 w2.
+  induction w1 as [|e w1 IHw1].
+  - reflexivity.
+  - simpl. rewrite IHw1. omega.
+Qed.
+
+Lemma count_buffer_distr' : forall w e,
+  count_buffer (w ++ [e]) = count_buffer w + count_event e.
+Proof.
+  intros w e.
+  rewrite count_buffer_distr.
+  simpl.
+  omega.
+Qed.
+
+Axiom upper_bound : Z.
+(* Definition upper_bound := 100. *)
+
+Definition upper_bounded := forall w, is_generated w -> count_buffer w <= upper_bound.
+
+Definition is_tangible q := ~ is_sink_state q /\ exists w, q = ixtransition w.
+
+Lemma buffer_count_leq_f : forall (f:state->Z),
+  ( f(0%nat) = 0 /\ forall q, is_tangible q -> forall e,
+    is_proper_transition q e -> f(xtransition q [e]) >= f(q) + count_event e )
+  -> forall w, is_generated w -> count_buffer w <= f(ixtransition w).
+Proof.
+  intros f [H H0] w H1.
+  induction w as [|e w IHw] using @rev_ind.
+  - simpl.
+    rewrite ixtransition_nil__0.
+    omega.
+  - pose H1 as H2; apply prefix_closed in H2.
+    apply IHw in H2.
+    rewrite ixtransition_distr.
+    rewrite count_buffer_distr'.
+    remember (ixtransition w) as q eqn:eq_q.
+    destruct (is_sink_stateb q) eqn:H3. {
+      apply is_sink_stateb__is_sink_state in H3.
+      apply prefix_closed in H1.
+      unfold is_generated in H1.
+      rewrite <- eq_q in H1.
+      contradiction.
+    }
+    remember (xtransition q [e]) as q' eqn:eq_q'.
+    destruct (is_sink_stateb q') eqn:H4. {
+      unfold is_generated in H1.
+      rewrite ixtransition_distr in H1.
+      rewrite <- eq_q, <- eq_q' in H1.
+      apply is_sink_stateb__is_sink_state in H4.
+      contradiction.
+    }
+    assert (f q' >= f q + count_event e). {
+      rewrite eq_q'.
+      apply H0.
+      - split.
+        + apply isnt_sink_stateb__isnt_sink_state in H3.
+          apply H3.
+        + exists w.
+          apply eq_q.
+      - unfold is_proper_transition.
+        rewrite <- eq_q'.
+        apply isnt_sink_stateb__isnt_sink_state.
+        apply H4.
+    }
+    omega.
+Qed.
+
+Theorem exists_function__upper_bounded :
+  ( exists f, f(0%nat) = 0 /\ forall q, is_tangible q -> 
+     f(q) <= upper_bound /\ (forall e,
+        is_proper_transition q e -> f(xtransition q [e]) >= f(q) + count_event e ))
+  -> upper_bounded.
+Proof.
+  unfold upper_bounded.
+  intros [f [H H0]] w H1.
+  assert (H2: count_buffer w <= f(ixtransition w)). {
+    apply buffer_count_leq_f; try split; try (apply H); try (apply H0); try (apply H1).
+  }
+  assert (f (ixtransition w) <= upper_bound). {
+    destruct (is_sink_stateb (ixtransition w)) eqn:H3.
+    - apply is_sink_stateb__is_sink_state in H3.
+      contradiction.
+    - destruct H0 with (q:=ixtransition w). {
+        split.
+          - apply isnt_sink_stateb__isnt_sink_state.
+            apply H3.
+          - exists w.
+            reflexivity.
+      }
+      apply H4.
+  }
+  omega.
+Qed.
+
 Fixpoint verify_upper_bound' (q:state) (m:Z) (s:list Z) (n:nat) :=
   match n with O => s | S n =>
 
     if (states_num <=? q)%nat then
         Return end_0 s
     else if nth q s (-1) =? -1 then
-        let s' := change s q m in
+        let s' := update s q m in
         Return max3_lists (verify_upper_bound' (transition q add) (m+1) s' n)
                           (verify_upper_bound' (transition q rem) (m-1) s' n)
                           (verify_upper_bound' (transition q oth)   m   s' n)
@@ -20,24 +131,27 @@ Fixpoint verify_upper_bound' (q:state) (m:Z) (s:list Z) (n:nat) :=
 
   end.
 
-Fixpoint verify_upper_bound'' (q:state) (m:Z) (s:list Z) (n:nat) :=
-  match n with O => s | S n =>
-
-    if (states_num <=? q)%nat then
-        Return end_0 s
-    else if nth q s (-1) =? -1 then
-        let s'   := change s q m in
-        let s''  := verify_upper_bound'' (transition q add) (m+1) s'  n in
-        let s''' := verify_upper_bound'' (transition q oth)   m   s'' n in
-        Return max3_lists s'' s''' (verify_upper_bound'' (transition q rem) (m-1) s''' n)
-    else if nth q s (-1) >=? m then
-        Return end_0 s
-    else
-        Return end_1 s
-
-  end.
-
 Definition verify_upper_bound :=
-  extract_0 (verify_upper_bound'' 0%nat 0 (initial_solution states_num) (states_num+2)) [].
+  extract_0 (verify_upper_bound' 0%nat 0 (initial_solution states_num) (states_num+2)) [].
 
-Compute verify_upper_bound.
+(* Compute verify_upper_bound. *)
+
+Definition state_upper_bound (q:state) := nth q (fst verify_upper_bound) (-1).
+
+Theorem upper_bounded__exists_function : upper_bounded ->
+  ( exists f, f(0%nat) = 0 /\ forall q, is_tangible q -> 
+     f(q) <= upper_bound /\ (forall e,
+        is_proper_transition q e -> f(xtransition q [e]) >= f(q) + count_event e )).
+Proof.
+  intro H.
+  exists state_upper_bound.
+Admitted.
+
+Theorem iff_exists_function__upper_bounded :
+  ( exists f, f(0%nat) = 0 /\ forall q, is_tangible q -> 
+     f(q) <= upper_bound /\ (forall e,
+        is_proper_transition q e -> f(xtransition q [e]) >= f(q) + count_event e ))
+  <-> upper_bounded.
+Proof.
+  split. apply exists_function__upper_bounded. apply upper_bounded__exists_function.
+Qed.
